Fixed HKDF

code/experimental/hkdf/Hacl.Impl.HKDF_SHA2_256.fst
@@ -17,23 +17,23 @@ module SpecSHA2 = Spec.SHA2
 module SpecHash = Spec.Hash
 module SpecHMAC = Spec.HMAC
 
-module Hash = Hacl.Impl.SHA2_256
-module HMAC = Hacl.Impl.HMAC_SHA2_256
+module Hash = Hacl.Hash.Definitions
+module HMAC = Hacl.HMAC
 
 
 inline_for_extraction noextract
-let a = Spec.SHA2.SHA2_256
+let a = Spec.Hash.Definitions.SHA2_256
 
-
+#set-options "--max_fuel 0 --max_ifuel 0"
 
 val hkdf_extract:
-    output: lbuffer uint8 (size (Spec.SHA2.size_hash a))
-  -> salt: buffer uint8 {length salt <= Spec.SHA2.max_input a}
+    output: lbuffer uint8 (size (Spec.Hash.Definitions.hash_length a))
+  -> salt: buffer uint8 {length salt <= Spec.Hash.Definitions.max_input_length a}
   -> slen: size_t{v slen == length salt}
   -> ikm: buffer uint8
   -> ilen: size_t{ v ilen == length ikm
-                /\ length salt + length ikm + Spec.SHA2.size_block a <= Spec.SHA2.max_input a
-                /\ Spec.SHA2.size_hash a + length ikm + Spec.SHA2.size_block a <= Spec.SHA2.max_input a} ->
+                /\ length salt + length ikm + Spec.Hash.Definitions.block_length a <= Spec.Hash.Definitions.max_input_length a
+                /\ Spec.Hash.Definitions.hash_length a + length ikm + Spec.Hash.Definitions.block_length a <= Spec.Hash.Definitions.max_input_length a} ->
   Stack unit
   (requires (fun h -> live h output /\ live h salt /\ live h ikm
                  /\ disjoint output salt /\ disjoint output ikm))
@@ -41,25 +41,26 @@ val hkdf_extract:
 
 let hkdf_extract output salt slen ikm ilen =
   push_frame ();
+  let hash_len = normalize_term(size (Spec.Hash.Definitions.hash_length a)) in
+  let salt0 = create hash_len  (u8 0) in
   admit();
-  let salt0 = create (size (Spec.SHA2.size_hash a)) (u8 0) in
-  (if slen = size 0 then
-    HMAC.hmac output salt0 (size (Spec.SHA2.size_hash a)) ikm ilen
-  else
-    HMAC.hmac output salt slen ikm ilen);
+  (if slen = size 0 then begin
+    HMAC.compute_sha2_256 output salt0 hash_len ikm ilen
+  end else
+    HMAC.compute_sha2_256 output salt slen ikm ilen);
   pop_frame()
 
 
 #reset-options "--z3rlimit 25"
 
 val hkdf_round0:
-    output: lbuffer uint8 (size (Spec.SHA2.size_hash a))
+    output: lbuffer uint8 (size (Spec.Hash.Definitions.hash_length a))
   -> prk: buffer uint8
-  -> plen: size_t{v plen == length prk /\ length prk <= Spec.SHA2.max_input a}
+  -> plen: size_t{v plen == length prk /\ length prk + Spec.Hash.Definitions.block_length a < max_size_t}
   -> info: buffer uint8
   -> ilen: size_t{ v ilen == length info
-                /\ length info + Spec.SHA2.size_hash a + 1 <= max_size_t
-                /\ length prk + length info + 1 + Spec.SHA2.size_hash a + Spec.SHA2.size_block a <= Spec.SHA2.max_input a} ->
+                /\ length info + Spec.Hash.Definitions.block_length a + 1 < max_size_t
+                /\ length prk + length info + 1 + Spec.Hash.Definitions.hash_length a + Spec.Hash.Definitions.block_length a <= Spec.Hash.Definitions.max_input_length a} ->
   Stack unit
   (requires (fun h -> live h output /\ live h prk /\ live h info
                  /\ disjoint output prk /\ disjoint output info))
@@ -67,35 +68,37 @@ val hkdf_round0:
 
 let hkdf_round0 output prk plen info ilen =
   push_frame ();
-  let input = create (ilen +. 1ul) (u8 0) in
-  update_sub #MUT #uint8 #(ilen +. 1ul) input (size 0) ilen info;
+  let input = create (ilen +! 1ul) (u8 0) in
+  update_sub #MUT #uint8 #(ilen +! 1ul) input (size 0) ilen info;
   upd input ilen (u8 1);
-  HMAC.hmac output prk plen input (ilen +. 1ul);
+  HMAC.compute_sha2_256 output prk plen input (ilen +! 1ul);
   pop_frame ()
 
 
 val hkdf_round:
-    output: lbuffer uint8 (size (Spec.SHA2.size_hash a))
+    output: lbuffer uint8 (size (Spec.Hash.Definitions.hash_length a))
   -> prk: buffer uint8
-  -> plen: size_t{v plen == length prk /\ length prk <= Spec.SHA2.max_input a}
+  -> plen: size_t{v plen == length prk /\ length prk + Spec.Hash.Definitions.block_length a < max_size_t}
   -> info: buffer uint8
   -> ilen: size_t{ v ilen == length info
-                /\ length info + Spec.SHA2.size_hash a + 1 <= max_size_t
-                /\ length prk + length info + 1 + Spec.SHA2.size_hash a + Spec.SHA2.size_block a <= Spec.SHA2.max_input a}
+                /\ length info + Spec.Hash.Definitions.hash_length a +
+		  Spec.Hash.Definitions.block_length a + 1 < max_size_t
+                /\ length prk + length info + 1 + Spec.Hash.Definitions.hash_length a + Spec.Hash.Definitions.block_length a <= Spec.Hash.Definitions.max_input_length a}
   -> i:size_t{1 < v i /\ v i <= 255}
-  -> ti: lbuffer uint8 (size (Spec.SHA2.size_hash a)) ->
+  -> ti: lbuffer uint8 (size (Spec.Hash.Definitions.hash_length a)) ->
   Stack unit
   (requires (fun h -> live h output /\ live h prk /\ live h info /\ live h ti
                  /\ disjoint output prk /\ disjoint output info /\ disjoint output ti))
   (ensures  (fun h0 _ h1 -> modifies1 output h0 h1))
 
 let hkdf_round output prk plen info ilen i ti =
+  let hash_len = normalize_term(size (Spec.Hash.Definitions.hash_length a)) in
   push_frame ();
-  let input = create (size (Spec.SHA2.size_hash a) +. ilen +. 1ul) (u8 0) in
-  update_sub input 0ul (size (Spec.SHA2.size_hash a)) ti;
-  update_sub #MUT #uint8 #(size (Spec.SHA2.size_hash a) +. ilen +. 1ul) input (size (Spec.SHA2.size_hash a)) ilen info;
-  upd #uint8 #(size (Spec.SHA2.size_hash a) +. ilen +. 1ul) input (size (Spec.SHA2.size_hash a) +. ilen) (to_u8 (size_to_uint32 i));
-  HMAC.hmac output prk plen input (size (Spec.SHA2.size_hash a) +. ilen +. 1ul);
+  let input = create (hash_len +! ilen +! 1ul) (u8 0) in
+  update_sub input 0ul hash_len ti;
+  update_sub #MUT #uint8 #(hash_len +! ilen +! 1ul) input hash_len ilen info;
+  upd #uint8 #(hash_len +! ilen +! 1ul) input (hash_len +! ilen) (to_u8 (size_to_uint32 i));
+  HMAC.compute_sha2_256 output prk plen input (hash_len +! ilen +! 1ul);
   pop_frame ()
 
 
@@ -104,14 +107,15 @@ let hkdf_round output prk plen info ilen i ti =
 val hkdf_expand:
     output: buffer uint8
   -> prk: buffer uint8
-  -> plen: size_t{v plen == length prk /\ length prk <= Spec.SHA2.max_input a}
+  -> plen: size_t{v plen == length prk /\ length prk + Spec.Hash.Definitions.block_length a < max_size_t}
   -> info: buffer uint8
   -> ilen: size_t{ v ilen == length info
-                /\ length info + Spec.SHA2.size_hash a + 1 <= max_size_t
-                /\ length prk + length info + 1 + Spec.SHA2.size_hash a + Spec.SHA2.size_block a <= Spec.SHA2.max_input a}
+                /\ length info + Spec.Hash.Definitions.hash_length a +
+		  Spec.Hash.Definitions.block_length a + 1 < max_size_t
+                /\ length prk + length info + 1 + Spec.Hash.Definitions.hash_length a + Spec.Hash.Definitions.block_length a <= Spec.Hash.Definitions.max_input_length a}
   -> len: size_t{ v len == length output
-               /\ v len + Spec.SHA2.size_hash a <= max_size_t
-               /\ v len / (Spec.SHA2.size_hash a) + 2 <= 255} ->
+               /\ v len + Spec.Hash.Definitions.hash_length a <= max_size_t
+               /\ v len / (Spec.Hash.Definitions.hash_length a) + 2 <= 255} ->
   Stack unit
   (requires (fun h -> live h output /\ live h prk /\ live h info
                  /\ disjoint output prk /\ disjoint output info))
@@ -119,9 +123,10 @@ val hkdf_expand:
 
 let hkdf_expand output prk plen info ilen len =
   push_frame ();
-  let n : size_t = len /. (size (Spec.SHA2.size_hash a)) +. 1ul in
-  let t = create (n *. size (Spec.SHA2.size_hash a)) (u8 0) in
-  let t0 = sub t (size 0) (size (Spec.SHA2.size_hash a)) in
+  let hash_len = normalize_term(size (Spec.Hash.Definitions.hash_length a)) in
+  let n : size_t = len /. hash_len +. 1ul in
+  let t = create (n *. hash_len) (u8 0) in
+  let t0 = sub t (size 0) hash_len in
   (* Compute T(0) *)
   hkdf_round0 t0 prk plen info ilen;
   (* Compute T(1) ... T(N)*)
@@ -129,8 +134,8 @@ let hkdf_expand output prk plen info ilen len =
   let h0 = ST.get () in
   loop_range_nospec #h0 (size 2) (n -. 1ul) t
     (fun i ->
-       let ti0 = sub t ((i -. 2ul) *. size (Spec.SHA2.size_hash a)) (size (Spec.SHA2.size_hash a)) in
-       let ti1 = sub t ((i -. 1ul) *. size (Spec.SHA2.size_hash a)) (size (Spec.SHA2.size_hash a)) in
+       let ti0 = sub t ((i -. 2ul) *. hash_len) hash_len in
+       let ti1 = sub t ((i -. 1ul) *. hash_len) hash_len in
        hkdf_round ti1 prk plen info ilen i ti0
     );
   let res = sub t (size 0) len in
@@ -146,9 +151,14 @@ val hkdf_build_label:
   -> llen: size_t{length label == v llen}
   -> context: buffer uint8
   -> clen: size_t{length context == v clen}
-  -> len: size_t{numbytes U16 + numbytes U8 + v llen + numbytes U8 + v clen <= max_size_t} ->
+  -> len: size_t{numbytes U16 + numbytes U8 + v llen + numbytes U8 + v clen <= max_size_t /\
+    length output >= numbytes U16 + numbytes U8 + v llen + numbytes U8 + v clen /\
+    v len < maxint U16
+  } ->
   Stack unit
-  (requires (fun h -> live h secret /\ live h label /\ live h context /\ live h output))
+  (requires (fun h -> live h secret /\ live h label /\ live h context /\ live h output /\
+    disjoint output label /\ disjoint output context
+  ))
   (ensures  (fun h0 _ h1 -> modifies1 output h0 h1))
 
 let hkdf_build_label output secret label llen context clen len =
@@ -160,24 +170,32 @@ let hkdf_build_label output secret label llen context clen len =
   let pos_clen: size_t = pos_label +. llen in
   let sz_clen: size_t = size (numbytes U8) in
   let pos_context: size_t = pos_clen +. sz_clen in
-  let vout = v sz_len + v sz_llen + v llen + v sz_clen + v clen in
-  update_sub #MUT #uint8 #vout output pos_len sz_len (uint_to_bytes_be #U8 #SEC (u16 len));
-  update_sub #MUT #uint8 #vout output pos_llen sz_llen (uint_to_bytes_be #U8 #SEC (u8 llen));
+  let vout = sz_len +! sz_llen +! llen +! sz_clen +! clen in
+  assert(v vout <= length output);
+  let output = LowStar.Buffer.sub output (size 0) vout in
+  uint_to_bytes_be #U16 #SEC (sub #MUT #uint8 #vout output pos_len sz_len) (to_u16 len);
+  uint_to_bytes_be #U8 #SEC (sub #MUT #uint8 #vout output pos_llen sz_llen) (to_u8 llen);
   update_sub #MUT #uint8 #vout output pos_label llen label;
-  update_sub #MUT #uint8 #vout output pos_clen sz_clen (uint_to_bytes_be #U8 #SEC (u8 clen));
+  uint_to_bytes_be #U8 #SEC (sub #MUT #uint8 #vout output pos_clen sz_clen) (to_u8 clen);
   update_sub #MUT #uint8 #vout output pos_context clen context
 
 
 val hkdf_expand_label:
     output: buffer uint8
-  -> secret: buffer uint8
+  -> secret: lbuffer uint8 (size 32)
   -> label: buffer uint8
   -> llen: size_t{length label == v llen}
   -> context: buffer uint8
   -> clen: size_t{length context == v clen}
-  -> len: size_t{numbytes U16 + numbytes U8 + v llen + numbytes U8 + v clen <= max_size_t /\ length output == v len} ->
+  -> len: size_t{numbytes U16 + numbytes U8 + v llen + numbytes U8 + v clen + v len +
+    Spec.Hash.Definitions.hash_length a + 1 + Spec.Hash.Definitions.block_length a < max_size_t /\
+    length output == v len /\ v len < maxint U16 /\
+    v len / (Spec.Hash.Definitions.hash_length a) + 2 <= 255
+  } ->
   Stack unit
-  (requires (fun h -> live h output /\ live h secret /\ live h label /\ live h context))
+  (requires (fun h -> live h output /\ live h secret /\ live h label /\ live h context /\
+    disjoint output secret /\ disjoint output label /\ disjoint output context
+  ))
   (ensures  (fun h0 _ h1 -> modifies1 output h0 h1))
 
 let hkdf_expand_label output secret label llen context clen len =
@@ -185,13 +203,15 @@ let hkdf_expand_label output secret label llen context clen len =
   let sz_len: size_t = size (numbytes U16) in
   let sz_llen: size_t = size (numbytes U8) in
   let sz_clen: size_t = size (numbytes U8) in
-  let ilabel = create (len +. sz_llen +. llen +. sz_clen +. clen) (u8 0) in
+  let ilen = sz_len +! sz_llen +! llen +! sz_clen +! clen in
+  let ilabel = create ilen (u8 0) in
+  let ilabel : buffer uint8 = ilabel in
   hkdf_build_label ilabel secret label llen context clen len;
-  hkdf_expand output secret 32ul ilabel (len +. sz_llen +. llen +. sz_clen +. clen) len;
+  assert_norm(32 + pow2 32 + 1000 < pow2 61);
+  hkdf_expand output secret (size 32) ilabel ilen len;
   pop_frame ()
 
 
 (* let hkdf_expand_derive_secret a secret label context = *)
 (*   let loghash = Hash.hash a context in *)
 (*   hkdf_expand_label a secret label loghash (Hash.size_hash a) *)
-
