code/experimental/hkdf/Hacl.HKDF_SHA2_256.fsti
@@ -15,40 +15,41 @@ module Loops = Lib.LoopCombinators
 
 
 inline_for_extraction noextract
-let a = Spec.SHA2.SHA2_256
+let a = Spec.Hash.Definitions.SHA2_256
 
 
 
 val hkdf_extract:
-    output: buffer uint8{length output == Spec.SHA2.size_hash a}
-  -> salt: buffer uint8 {length salt <= Spec.SHA2.max_input a}
+    output: buffer uint8{length output == Spec.Hash.Definitions.hash_length a}
+  -> salt: buffer uint8 {length salt <= Spec.Hash.Definitions.max_input_length a}
   -> slen: size_t{v slen == length salt}
   -> ikm: buffer uint8
   -> ilen: size_t{ v ilen == length ikm
-                /\ length salt + length ikm + Spec.SHA2.size_block a <= Spec.SHA2.max_input a
-                /\ Spec.SHA2.size_hash a + length ikm + Spec.SHA2.size_block a <= Spec.SHA2.max_input a} ->
+                /\ length salt + length ikm + Spec.Hash.Definitions.block_length a <= Spec.Hash.Definitions.max_input_length a
+                /\ Spec.Hash.Definitions.hash_length a + length ikm + Spec.Hash.Definitions.block_length a <= Spec.Hash.Definitions.max_input_length a} ->
   Stack unit
   (requires (fun h -> live h output /\ live h salt /\ live h ikm
                  /\ disjoint output salt /\ disjoint output ikm))
   (ensures  (fun h0 _ h1 -> modifies1 output h0 h1))
 
 
+
 val hkdf_expand:
     output: buffer uint8
   -> prk: buffer uint8
-  -> plen: size_t{v plen == length prk /\ length prk <= Spec.SHA2.max_input a}
+  -> plen: size_t{v plen == length prk /\ length prk + Spec.Hash.Definitions.block_length a < max_size_t}
   -> info: buffer uint8
   -> ilen: size_t{ v ilen == length info
-                /\ length info + Spec.SHA2.size_hash a + 1 <= max_size_t
-                /\ length prk + length info + 1 + Spec.SHA2.size_hash a + Spec.SHA2.size_block a <= Spec.SHA2.max_input a}
+                /\ length info + Spec.Hash.Definitions.hash_length a +
+		  Spec.Hash.Definitions.block_length a + 1 < max_size_t
+                /\ length prk + length info + 1 + Spec.Hash.Definitions.hash_length a + Spec.Hash.Definitions.block_length a <= Spec.Hash.Definitions.max_input_length a}
   -> len: size_t{ v len == length output
-               /\ v len + Spec.SHA2.size_hash a <= max_size_t
-               /\ v len / (Spec.SHA2.size_hash a) + 2 <= 255} ->
+               /\ v len + Spec.Hash.Definitions.hash_length a <= max_size_t
+               /\ v len / (Spec.Hash.Definitions.hash_length a) + 2 <= 255} ->
   Stack unit
   (requires (fun h -> live h output /\ live h prk /\ live h info
                  /\ disjoint output prk /\ disjoint output info))
   (ensures  (fun h0 _ h1 -> modifies1 output h0 h1))
-
 
 val hkdf_build_label:
     output: buffer uint8
@@ -57,20 +58,31 @@ val hkdf_build_label:
   -> llen: size_t{length label == v llen}
   -> context: buffer uint8
   -> clen: size_t{length context == v clen}
-  -> len: size_t{numbytes U16 + numbytes U8 + v llen + numbytes U8 + v clen <= max_size_t} ->
+  -> len: size_t{numbytes U16 + numbytes U8 + v llen + numbytes U8 + v clen <= max_size_t /\
+    length output >= numbytes U16 + numbytes U8 + v llen + numbytes U8 + v clen /\
+    v len < maxint U16
+  } ->
   Stack unit
-  (requires (fun h -> live h secret /\ live h label /\ live h context /\ live h output))
+  (requires (fun h -> live h secret /\ live h label /\ live h context /\ live h output /\
+    disjoint output label /\ disjoint output context
+  ))
   (ensures  (fun h0 _ h1 -> modifies1 output h0 h1))
 
 
 val hkdf_expand_label:
     output: buffer uint8
-  -> secret: buffer uint8
+  -> secret: lbuffer uint8 (size 32)
   -> label: buffer uint8
   -> llen: size_t{length label == v llen}
   -> context: buffer uint8
   -> clen: size_t{length context == v clen}
-  -> len: size_t{numbytes U16 + numbytes U8 + v llen + numbytes U8 + v clen <= max_size_t /\ length output == v len} ->
+  -> len: size_t{numbytes U16 + numbytes U8 + v llen + numbytes U8 + v clen + v len +
+    Spec.Hash.Definitions.hash_length a + 1 + Spec.Hash.Definitions.block_length a < max_size_t /\
+    length output == v len /\ v len < maxint U16 /\
+    v len / (Spec.Hash.Definitions.hash_length a) + 2 <= 255
+  } ->
   Stack unit
-  (requires (fun h -> live h output /\ live h secret /\ live h label /\ live h context))
+  (requires (fun h -> live h output /\ live h secret /\ live h label /\ live h context /\
+    disjoint output secret /\ disjoint output label /\ disjoint output context
+  ))
   (ensures  (fun h0 _ h1 -> modifies1 output h0 h1))
