specs/Spec.HKDF.fsti
@@ -11,9 +11,9 @@ module HMAC = Spec.HMAC
 
 val hkdf_extract:
     a:Hash.hash_alg
-  -> salt: bytes{length salt < Hash.max_input_length a}
-  -> ikm: bytes{length salt + length ikm + Hash.block_length a < Hash.max_input_length a
-        /\ Hash.hash_length a + length ikm + Hash.block_length a < Hash.max_input_length a} ->
+  -> salt: bytes{length salt  + Hash.block_length a < Hash.max_input_length a}
+  -> ikm: bytes{length salt + length ikm + Hash.block_length a < max_size_t
+        /\ Hash.hash_length a + length ikm + Hash.block_length a < max_size_t} ->
   Tot (lbytes (Hash.hash_length a))
 
 
@@ -21,7 +21,7 @@ val hkdf_expand:
     a:Hash.hash_alg
   -> prk:bytes{length prk < Hash.max_input_length a}
   -> info: bytes{length info + Hash.hash_length a + 1 < max_size_t (* BB. FIXME, this is required by create *)
-              /\ length prk + length info + 1 + Hash.hash_length a + Hash.block_length a < Hash.max_input_length a}
+              /\ length prk + length info + 1 + Hash.hash_length a + Hash.block_length a < max_size_t}
   -> len:size_nat{len < 255 * Hash.hash_length a} ->
   Tot (lbytes len)
 
@@ -41,11 +41,10 @@ val hkdf_expand_label:
   -> label: bytes{length label <= maxint U8}
   -> context: bytes{
     let size_hkdf_label = numbytes U16 + numbytes U8 + length label + numbytes U8 + length context in
-    length context <= maxint U8
-  /\ length secret + size_hkdf_label + 1 + Hash.hash_length a + Hash.block_length a < Hash.max_input_length a}
+    length context < maxint U8
+  /\ length secret + size_hkdf_label + 1 + Hash.hash_length a + Hash.block_length a < max_size_t}
   -> len: nat{len <= maxint U16 /\ len < 255 * Hash.hash_length a} ->
   Tot (lbytes len)
-
 
 val hkdf_expand_derive_secret:
     a: Hash.hash_alg
@@ -54,5 +53,5 @@ val hkdf_expand_derive_secret:
   -> context: bytes{
     let size_hkdf_label = numbytes U16 + numbytes U8 + length label + numbytes U8 + Hash.hash_length a in
     length context <= maxint U8
-  /\ length secret + size_hkdf_label + 1 + Hash.hash_length a + Hash.block_length a < Hash.max_input_length a} ->
+  /\ length secret + size_hkdf_label + 1 + Hash.hash_length a + Hash.block_length a < max_size_t} ->
   Tot (lbytes (Hash.hash_length a))
